tests/GAST.v
@@ -21,10 +21,10 @@ Time Autosubst Generate.
 (** *** Glue code (eventually should be generic). *)
 (*********************************************************************************)
 
-(** Solve a goal of the form [Simplification term t0 _]. *)
+(** Solve a goal of the form [TermSimplification t0 _]. *)
 Ltac2 solve_term_simplification () : unit :=
   lazy_match! Control.goal () with 
-  | Simplification term ?t0 _ =>
+  | TermSimplification ?t0 _ =>
     (* Reify Level 0 -> Level 1. *)
     let (t1, p1) := reify_term t0 in 
     printf "t1: %t" t1;
@@ -54,65 +54,77 @@ Ltac2 solve_term_simplification () : unit :=
       (eq_sym $p1) 
       (eq_trans (f_equal (eval Sig.Kt) $eq1) $p3)) 
     in
-    exact (MkSimplification term $t0 $t0' $eq)
+    exact (MkTermSimplification _ $t0 $t0' $eq)
   | _ => Control.zero (Tactic_failure None)
   end.
 
-(*Lemma congr_seval {s1 s2} : 
+Lemma congr_seval {s1 s2} : 
   s1 =₁ s2 -> seval s1 =₁ seval s2.
 Proof. intros H i. unfold seval. now rewrite H. Qed. 
 
 (** Solve a goal of the form [Simplification subst s0 _]. *)
 Ltac2 solve_subst_simplification () : unit :=
   lazy_match! Control.goal () with 
-  | Simplification subst ?s0 _ =>
+  | SubstSimplification ?s0 _ =>
+    printf "Simplifying substitution: %t" s0;
     (* Reify Level 0 -> Level 1. *)
     let (s1, p1) := reify_subst s0 in 
     (* Reify Level 1 -> Level 2. *)
     let env := T.empty_env () in
-    let (env, s2) := T.reify_subst env s1 in
-    let env := T.build_env env in
+    let (env, s2) := T.reify_subst constr:(sig) env s1 in
+    let env := T.build_env constr:(sig) env in
     (* Simplify on Level 2. *)
-    let s2' := Std.eval_cbv (T.red_flags_simp ()) constr:(T.ssimp $s2) in
-    let s2'' := Std.eval_cbv (T.red_flags_clean ()) constr:(T.sclean $s2') in
+    let s2' := Std.eval_cbv (red_flags_simp ()) constr:(Simp.ssimp $s2) in
+    let s2'' := Std.eval_cbv (red_flags_clean ()) constr:(Clean.sclean $s2') in
     (* Eval Level 2 -> Level 1. *)
-    let s1' := Std.eval_cbv (T.red_flags_eval ()) constr:(T.seval $env $s2'') in
+    let s1' := Std.eval_cbv (red_flags_eval ()) constr:(T.seval $env $s2'') in
     (* Eval Level 1 -> Level 0. *)
     let (s0', p3) := eval_subst s1' in
-    (* [eq1 : s1 =₁ s1']. *)
-    let eq1 := constr:(transitivity
-      (symmetry (T.ssimp_sound $env $s2))
-      (symmetry (T.sclean_sound $env $s2'))) 
+    (* [peq1 : s1 =₁ s1']. *)
+    let peq1 := constr:(transitivity
+      (Simp.sred_sound $env _ _ (Simp.ssimp_red $s2))
+      (Clean.sred_sound $env _ _ (Clean.sclean_red $s2'))) 
     in
-    (* [eq0 : s0 =₁ s0']. *)
-    let eq := constr:(transitivity
+    (* [peq0 : s0 =₁ s0']. *)
+    let peq0 := constr:(transitivity
       (symmetry $p1) 
-      (transitivity (congr_seval $eq1) $p3)) 
+      (transitivity (congr_seval $peq1) $p3)) 
     in
-    exact (MkSimplification subst $s0 $s0' $eq)
-  | _ => Control.zero (Tactic_failure None) 
-  end.*)
+    exact (MkSubstSimplification _ $s0 $s0' $peq0)
+  | _ => Control.zero (Tactic_failure None)
+  end.
+
+(** Solve a goal of the form [Simplification _ _ _] or [PSimplification _ _ _]. *)
+Ltac solve_simplification :=
+  solve [ ltac2:(solve_term_simplification ()) 
+        | ltac2:(solve_subst_simplification ()) ].
+
+Ltac rasimpl_topdown := 
+  (rewrite_strat (topdown (hints asimpl_topdown))) ; [| solve_simplification ..].
+
+Ltac rasimpl_outermost := 
+  (rewrite_strat (outermost (hints asimpl_outermost))) ; [| solve_simplification ..].
 
 (** Main simplification tactic. *)
 Ltac rasimpl := 
-  (try rewrite_strat (topdown (hints asimpl))) ; 
-  [ |ltac2:(solve_term_simplification ()) (*| ltac2:(solve_subst_simplification ()*) ..].
+  repeat rasimpl_topdown ;
+  repeat rasimpl_outermost.
 
-(** Trigger for [rasimpl]. *)
+(** Trigger [rasimpl] on [rename _ _]. *)
 Lemma autosubst_simpl_term_rename (r : ren) (t res : term) :
-  Simplification term (rename r t) res -> rename r t = res.
-Proof. intros H. now apply simplification. Qed.
-#[export] Hint Rewrite -> autosubst_simpl_term_rename : asimpl.
+  TermSimplification (rename r t) res -> rename r t = res.
+Proof. intros H. now apply term_simplification. Qed.
+#[export] Hint Rewrite -> autosubst_simpl_term_rename : asimpl_topdown.
 
-(** Trigger for [rasimpl]. *)
+(** Trigger [rasimpl] on [substitute _ _]. *)
 Lemma autosubst_simpl_term_substitute (s : subst) (t res : term) :
-  Simplification term (substitute s t) res -> substitute s t = res.
-Proof. intros H. now apply simplification. Qed.
-#[export] Hint Rewrite -> autosubst_simpl_term_substitute : asimpl.
+  TermSimplification (substitute s t) res -> substitute s t = res.
+Proof. intros H. now apply term_simplification. Qed.
+#[export] Hint Rewrite -> autosubst_simpl_term_substitute : asimpl_topdown.
 
 Axiom r : ren.
 Axiom s : subst.
 Axiom t : term.
 Axiom i : nat.
-Lemma test : rename (rcons (r 0) (rcomp rshift r)) (Var i) = Var 0.
-Proof. rasimpl. Admitted.
+Lemma test : substitute (scomp sshift (scons (Var 0) sid)) t = Var 0.
+Proof. rasimpl_topdown. Admitted.
